Add InOut for dynamic input / output parameters of proof mode classes
This commit adds [InOut] that is used to dynamically determine whether
a type class parameter is an input or an output. This is important for
classes that are used with multiple modings, e.g., IntoWand. Instances
can match on the InOut parameter to avoid accidentially instantiating
outputs if matching on an input was intended.

src/Iris/ProofMode/Classes.lean
@@ -9,6 +9,15 @@ import Iris.ProofMode.SynthInstance
 namespace Iris.ProofMode
 open Iris.BI
 
+/-- [InOut] is used to dynamically determine whether a type class
+parameter is an input or an output. This is important for classes that
+are used with multiple modings, e.g., IntoWand. Instances can match on
+the InOut parameter to avoid accidentially instantiating outputs if
+matching on an input was intended. -/
+inductive InOut where
+  | in
+  | out
+
 inductive AsEmpValid.Direction where
   | into
   | from
@@ -40,7 +49,9 @@ class FromWand [BI PROP] (P : PROP) (Q1 Q2 : outParam PROP) where
 export FromWand (from_wand)
 
 @[ipm_class]
-class IntoWand [BI PROP] (p q : Bool) (R : PROP) (P Q : outParam PROP) where
+class IntoWand [BI PROP] (p q : Bool) (R : PROP)
+  (ioP : InOut) (P : semiOutParam PROP)
+  (ioQ : InOut) (Q : semiOutParam PROP) where
   into_wand : □?p R ⊢ □?q P -∗ Q
 export IntoWand (into_wand)
 
@@ -112,7 +123,7 @@ export IntoAbsorbingly (into_absorbingly)
 
 
 @[ipm_class]
-class FromAssumption (p : Bool) [BI PROP] (P : semiOutParam PROP) (Q : PROP) where
+class FromAssumption (p : Bool) [BI PROP] (ioP : InOut) (P : semiOutParam PROP) (Q : PROP) where
   from_assumption : □?p P ⊢ Q
 export FromAssumption (from_assumption)
 
